\noindent The sensor can be described by the first-order differential equation 
\begin{equation}
a_{\text{0}}x+a_{\text{1}}\dot{x}=bu
\end{equation}
\noindent From the questions $a_{\text{0}}\neq0$
\begin{equation}
x+\frac{a_{\text{1}}}{a_{\text{0}}}\dot{x}=\frac{b}{a_{\text{0}}}u
\end{equation}
\noindent Substitute time constant $\tau=\frac{a_{\text{1}}}{a_{\text{0}}}$ and static gain $K=\frac{b}{a_{\text{0}}}$ into the equation.
\begin{equation}
x+\tau\dot{x}=Ku
\end{equation}
\noindent Apply the Laplace transform on the both sides of the equation assuming zero initial conditions
\begin{equation}
(1+{\tau}s)X(s)=KU(s)
\end{equation}
\noindent Therefore, the transfer function of the sensor is
\begin{equation}
G(s)=\frac{X(s)}{U(s)}=\frac{K}{{\tau}s+1}
\end{equation}